\chapter{LATE (Local Average Treatment Effect)(COMING SOON)}
\label{ch-late}


The {\bf Local Average Treatment Effect (LATE)}


\begin{figure}[h!]
$$
\begin{array}{ccccc}
\xymatrix{
&&\rvx\ar[ddl]\ar[ddr]
\\
\\
\rva\ar[r]
&\rvd\ar[rr]&&\rvy
}
&
\xymatrix{
&&\rvx\ar[dl]\ar[dr]
\\
&
[\rvd(a')]_{a'=0}^1\ar[d]
&
&[\rvy(d')]_{d'=0}^1\ar[d]
\\
\rva\ar[r]
&\rvd\ar[rr]&&\rvy
}
\\
G
&
G_+=
\cali_{\rvd\rarrow \rvy}
\cali_{\rva\rarrow \rvd}G
\end{array}
$$
\caption{
Bnet $G_+$ is bnet $G$
after application of 2
imagine operators.
Imagine operators
are discussed in Chapter \ref{ch-counterf}.
}
\label{fig-late-g-gplus}
\end{figure}

% Please add the following required packages to your document preamble:
% \usepackage[table,xcdraw]{xcolor}
% If you use beamer only pass "xcolor=table" option, i.e. \documentclass[xcolor=table]{beamer}
\begin{table}[h!]
\centering
\begin{tabular}{|l|l|l|}
\hline
 & \cellcolor[HTML]{ECF4FF}$d^\s(0)$ & \cellcolor[HTML]{ECF4FF}$d^\s(1)$ \\ \hline
\cellcolor[HTML]{ECF4FF}never-takers & 0 & 0 \\ \hline
\cellcolor[HTML]{ECF4FF}compliers & 0 & 1 \\ \hline
\cellcolor[HTML]{ECF4FF}defiers & 1 & 0 \\ \hline
\cellcolor[HTML]{ECF4FF}always-takers & 1 & 1 \\ \hline
\end{tabular}
\caption{Possible compliance
behaviors  for individual $\s$.}
\label{tab-late compliance}
\end{table}

\beq\color{blue}
P(d|a,
[d(a')]_{a'=0}^1
) = \indi(\quad
d= \underbrace
{a d(a) + (1-a)d(1-a)}
_{\sum_{a'=0}^1
\delta(a,a')d(a')}
\quad)
\eeq

\beq\color{blue}
P(y|d,
[y(d')]|_{d'=0}^1)
= \indi(\quad
y= \sum_{d'=0}^{1}
\delta(d,d')
y(d')
\quad)
\eeq


\beq
\cald_{|a} = \sum_d d\; P(d|a)
\eeq

\beq
\caly_{|d,a}=\sum_y y\;P(y|d,a)
=
E_{|d,a}[\rvy]
\eeq

\beq
\caly_{|\rvd=d}=\sum_y y\;P(y|d)
= E_{|d}[\rvy]
\eeq

\beq
\caly_{|\rva=a}=
\sum_y y\;P(y|a)
=
E_{|a}[\rvy]
\eeq

monotonicity
\beq
d^\s(1)
\geq
 d^\s(0)
\eeq
rules out defiers
(i.e., 
$d^\s(1)=0,
\;
d^\s(0)=1$)

Assume that $
\cald_{|1}\neq\cald_{|0}
$. Then
LATE is defined by

\beq
LATE = \frac{\caly_{|\rva=1}-
\caly_{|\rva=0}}
{\cald_{|1}-\cald_{|0}}
\eeq

Complier
\beq
\calc=\{\rvd(0)=0, \rvd(1)=1\}
\eeq 

\begin{claim}
If monotonicity is satisfied, then

\beq
P(\calc)=
\cald_{|1}-\cald_{|0}
\eeq
\end{claim}
\proof
\beqa
\cald_{|1}-\cald_{|0}
&=&
\sum_{d(0), d(1)}
P(d(0), d(1))[d(1)-d(0)]
\\
&=&
\left\{
\begin{array}{r}
P(d(0)=0, d(1)=0)
\underbrace{[d(1)-d(0)]}_{0}
\\
+P(d(0)=0, d(1)=1)
\underbrace{[d(1)-d(0)]}
_{1}
\\
+\underbrace{P(d(0)=1, d(1)=0)}
_{=0 \text{ by monotonicity}}
[d(1)-d(0)]
\\
+P(d(0)=1, d(1)=1)
\underbrace{[d(1)-d(0)]}_{0}
\end{array}
\right.
\\
&=& P(\calc)
\eeqa

\qed


\begin{claim}
If monotonicity is satisfied, then

\beq
LATE=
E_{|\calc}[\rvy(1)-\rvy(0)]
\eeq
 
\end{claim}
\proof

\begin{align}
\caly_{|\rva=1}-
\caly_{|\rva=0}
&=
E_{|\rva=1}[\rvy]
-
E_{|\rva=0}[\rvy]
\\
&=
\sum_x
\sum_{y(0), y(1)}
\sum_{d(0), d(1)}
\left\{
\begin{array}{l}
[y(d(1))-y(d(0))]
\\
*P(y(0), y(1)|x)
\\
*P(d(0), d(1)|x)
\\
*P(x)
\end{array}
\right.
\\
&=
\sum_{y(0), y(1)}
\sum_{d(0), d(1)}
[y(d(1))-y(d(0))]
\left\{
\begin{array}{l}
P(y(0), y(1)|d(0), d(1))
\\
*P(d(0), d(1))
\end{array}
\right.
\\
&=
\sum_{y(0), y(1)}
\left\{
\begin{array}{r}
\underbrace{[y(0)-y(0)]}_{0}
\left\{
\begin{array}{l}
P(y(0), y(1)|d(0)=0, d(1)=0)
\\
*P(d(0)=0, d(1)=0)
\end{array}
\right.
\\
\\
+
[y(1)-y(0)]
\left\{
\begin{array}{l}
P(y(0), y(1)|d(0)=0, d(1)=1)
\\
*P(d(0)=0, d(1)=1)
\end{array}
\right.
\\
\\
+
[y(0)-y(1)]
\left\{
\begin{array}{l}
P(y(0), y(1)|d(0)=0, d(1)=0)
\\
*\underbrace{P(d(0)=0, d(1)=0)}
_{=0 \text{  monotonicity}}
\end{array}
\right.
\\
\\
+
\underbrace{[y(1)-y(1)]}_{0}
\left\{
\begin{array}{l}
P(y(0), y(1)|d(0)=1, d(1)=1)
\\
*P(d(0)=1, d(1)=1)
\end{array}
\right.
\end{array}
\right.
\\
&=
P(\calc)
\sum_{y(0), y(1)}
[y(1)-y(0)]
P(y(0), y(1)|\calc)
\\
&=
P(\calc)
E_{|\calc}[\rvy(1)-\rvy(0)]
\end{align}
\qed
