\chapter{Stochastic Differential Equations COMING SOON}
\label{ch-stochastic-diff-eqns}

Stochastic Differential Equation (SDE)
First order differential equation with noise

Ref.\cite{sde-applied-book}

\section{Notation}

$[n]=[0:n]=\{0, 1, 2, \ldots, n-1\}$

$dx^n = dx_0 dx_1 \ldots dx_{n-1}$

\beq 
\av{\rva} = E[\rva]
\eeq

\beq
\Delta \rva = \rva - \av{\rva}
\eeq

\beq
Cov(\rva, \rvb) =\av{\rva, \rvb}=
\av{\Delta\rva \Delta\rvb}
\eeq

\beq
\Delta_{t_0}^{t_1}a = a(t_1) - a(t_0)
\eeq



random process $\rvx(t)$ for $t\geq 0$

$t_0=0 < t_1 < t_2 <\ldots< t_{N-1}$

sequence of random variables $\rvx(t_0),
 \rvx(t_1), \rvx(t_2), \ldots \rvx(t_{N-1})$
 
Will often define $\rvx(t_i) =\rvx_i$.

Will use lower case Latin indices for time
and Greek letters for $\rvx\in\RR^n$ components.
Hence $\rvx_{\mu, i}=\rvx_\mu(t_i)$



 
 \section{White Noise and Brownian Motion}
 
 \begin{figure}[h!]
 \centering
 \includegraphics[width=4in]
 {stochastic-diff-eqns/white-noise-labeled}
 \caption{One dimensional white noise $\rvW(t)$}
 \label{fig-white-noise-t}
 \end{figure}
 
 \begin{figure}[h!]
  \centering
  \includegraphics[width=4in]
  {stochastic-diff-eqns/brownian-motion-labeled}
  \caption{One dimensional Brownian motion $\rvB(t)$}
  \label{fig-brownian-motion-t}
  \end{figure}
  
 

White noise $\rvW(t)
\in\RR^n$ for $t\geq 0$

\begin{enumerate}
\item
\beq
\rvW(t) \sim \caln(\mu=0, Cov=Q)
\eeq

\item
$\rvW(t)$ and $\rvW(s)$ independent for
$t\neq s$

\item

\beq E[\rvW(t)]=0
\eeq

\item
\beq
C_\rvW(t, s) = \av{\rvW(t), \rvW^T(s)} = Q\delta(t-s)
\eeq



\end{enumerate}
Brownian motion (a.k.a. as a Wiener process) $\rvB\in\RR^n$
for $t\geq 0$

\begin{enumerate}

\item

\beq 
\rvB(0)=0\footnote{For $\rvB(0)=\beta_0\neq 0$, replace
$\rvB$ by $\rvB-\beta_0$}
\eeq

\item

\beq
\frac{
\Delta_{t_k}^{t_{k+1}}\rvB
}{\Delta_{t_k}^{t_{k+1}}t}
\sim \caln(\mu=0, Cov=Q)
\eeq

\beq
\rvW(t_k)\sim  \caln(\mu=0, Cov=Q)
\eeq

\beq
\frac
{d \rvB}{dt} = \rvW
\eeq


\item

\beq
E[(\Delta^{r}_{s}\rvB)^2] = n|r-s|
\eeq
where $\rvB(t)\in\RR^n$


\item
If $[r, s]\cap [r', s']=\emptyset$ then

\beq
E[(\Delta^{s}_{r}\rvB) (\Delta^{s'}_{r'}\rvB)]=0
\eeq


\beqa
E[\Delta_1^4\rvB \Delta_3^6\rvB]
&=&
E[(\Delta_1^3\rvB + \Delta_3^4\rvB)
(\Delta_3^4\rvB + \Delta_4^6\rvB)
]
\\
&=&
E[(\Delta_3^4\rvB)^2]
\\
&=& n |4-3|
\eeqa

In general

\beq
E[(\Delta^{s}_{r}\rvB) (\Delta^{s'}_{r'}\rvB)]=n {\rm len}([r, s]\cap [r', s'])
\eeq

\end{enumerate}

\section{SDE bnet}

special nodes

We discussed marginalizer nodes in Chapter
\ref{ch-marginalizer}.

\begin{itemize}

\item {\bf diff ad diff0} 

$$\xymatrix{
\rva\ar[dr]
&&\rvb\ar[dl]
\\
&
\rvx
}
$$

\beq  \color{blue}
P(x|a, b) =\indi (x =a-b)
\eeq

\beq  \color{blue}
x =a-b
\eeq
 diff0 node is the diff node with $x=0$
 


\item {\bf accumulator}

$$
\xymatrix{
\rvx_3 \ar[d]
&\rvx_2\ar[d]
&\rvx_1\ar[d]
&\rvx_0\ar[d]
\\
\rvs_3 
&\rvs_2\ar[l]
 &\rvs_1\ar[l]
  &\rvs_0\ar[l]
}$$



\beq
\color{blue}
\begin{array}{lll}
\rvs_3 &=& \rvx_3 + \rvs_2
\\
\rvs_2 &=& \rvx_2 + \rvs_1
\\
\rvs_1 &=& \rvx_1 + \rvs_0
\\
\rvs_0&=& x_0
\end{array}
\eeq

\item {\bf incrementer}

$$
\xymatrix{
\rvB_3\ar[dr] 
&& \rvB_2\ar[dl]\ar[dr]
&& \rvB_1\ar[dl]\ar[dr]
&& \rvB_0\ar[dl]
\\
&\Delta^3_2\rvB 
&&\Delta^2_1 \rvB 
&&\Delta^1_0 \rvB
&
}$$

\beq\color{blue}
\begin{array}{lll}
\Delta_2^3\rvB &=& \rvB_3 - \rvB_2
\\
\Delta_1^2\rvB &=& \rvB_2 - \rvB_1
\\
\Delta_0^1\rvB &=& \rvB_1 - \rvB_0
\end{array}
\eeq

\item {\bf de-incrementer}
$$
\xymatrix{
&\Delta^3_2\rvx_2 \ar[dl] 
&&\Delta^2_1 \rvx \ar[dlll]\ar[dl]
&&\Delta \rvx^1_0 \ar[dlllll]\ar[dlll]\ar[dl]
&
\\
\rvx_3 
&& \rvx_2 
&& \rvx_1
&& \rvx_0
\ar@/^1pc/[ll]
\ar@/^1pc/[llll]
\ar@/^1pc/[llllll]
}
$$
\beq
\color{blue}
\begin{array}{lll}
\rvx_3 &=& \Delta_2^3\rvx + \Delta_1^2\rvx
+ \Delta^1_0\rvx + x_0
\\
\rvx_2 &=& \Delta_1^2\rvx
+ \Delta^1_0\rvx + x_0
\\
\rvx_1 &=&
\Delta^1_0\rvx + x_0
\\
\rvx_0&=&x_0
\end{array}
\eeq
\end{itemize}


$\rvx, \rvB\in \RR$
\beq
d\rvx= f(\rvx, t)dt + L(\rvx, t)d\rvB(t)
\eeq

\begin{figure}
$$
\xymatrix{
\rvB_3\ar@[red][dr] 
&& \rvB_2\ar@[red][dl]\ar@[red][dr]
&& \rvB_1\ar@[red][dl]\ar@[red][dr]
&& \rvB_0\ar@[red][dl]
\\
&\Delta^3_2\rvB \ar[d]
&&\Delta^2_1 \rvB \ar[d]
&&\Delta^1_0 \rvB \ar[d]
&
\\
&\Delta^3_2\rvx \ar@[green][dl] 
&&\Delta^2_1 \rvx \ar@[green][dlll]\ar@[green][dl]
&&\Delta^1_0\rvx \ar@[green][dlllll]\ar@[green][dlll]\ar@[green][dl]
&
\\
\rvx_3 
&& \rvx_2 \ar[lu] 
&& \rvx_1 \ar[lu]
&& \rvx_0\ar[lu]
\ar@[green]@[green]@/^1pc/[ll]
\ar@[green]@/^1pc/[llll]
\ar@[green]@/^1pc/[llllll]
}
$$
\caption{Bnet for general SDE with $N=4$ number of times. Note that this bnet
contains within it first an incrementer bnet
(in red) for the $\rvB_i$
then a de-incrementer bnet (in green)
for the $\rvx_i$.}
\label{fig-sde-3-nodes}
\end{figure}


\beq
\color{blue}
\Delta_{2}^{3}\rvB = 
\rvB_3 -\rvB_2
\eeq

\beq
\color{blue}
\Delta_{2}^{3}\rvx = 
f(x_3, t)\Delta_2^3 t +
L(x_3, t)\Delta_{2}^{3}\rvB
\eeq

\beq\color{blue}
\rvx_3 = \Delta_{2}^{3}\rvx
+\Delta_{1}^{2}\rvx
+\Delta_{0}^{1}\rvx
+x_0
\eeq



\section{It\^{o} Integral}

Consider 1 dimensional case $\rvx, \rvW\in \RR$.
\beq
\frac{d\rvx}{dt}= f(\rvx, t) + L(\rvx, t)\rvW(t)
\eeq

\beq
\rvx(t) - \rvx(0) =
\int_{0}^{t}dt\; f(\rvx(t), t) + J
\eeq

\beq
J = \int_{0}^t dt\;
L(\rvx(t), t)\rvW(t)
\eeq

$t_0=0 < t_1 <\ldots <t_{N-1}$, $t_k^*\in [t_k, t_{k+1})$

\beq 
J = \lim_{N\rarrow \infty} J_N
\eeq


\beq 
J_N = 
\sum_k L(\rvx(t_k^*), t_k^*)\Delta_{t_k}^{t_{k+1}}\rvB
\eeq


Suppose $L=\rvx=\rvB$

\beq
J_N=\sum_k \rvB(t_k^*) \Delta_{t_k}^{t_{k+1}}\rvB
\eeq

\begin{enumerate}

\item $t_k^* = t_k$, Ito integral\footnote{More precisely,
It\^{o}}


\beqa
E[J_N] &=&\sum_k E[\rvB(t_k)\Delta_{t_k}^{t_{k+1}}\rvB] 
\\
&=& \sum_k
E[(\Delta_{0}^{t_k}\rvB)\Delta_{t_k}^{t_{k+1}}\rvB] 
\\
&=&0
\eeqa

\beqa
J_N &=& 
\sum_k \rvB(t_k)\Delta_{t_k}^{t_{k+1}}\rvB
\\
&=&
\frac{1}{2}\sum_k\left[
-[\Delta_{t_k}^{t_{k+1}}\rvB]^2
+ \Delta_{t_k}^{t_{k+1}}(\rvB^2)\right]
\eeqa

\beqa
J &=& \lim_{N\rarrow \infty} J_N
\\
&=&
\frac{1}{2}
(-t+\rvB^2(t))
\eeqa
$E[J] = \frac{1}{2}(-t+t)=0$



\item $t_k^* = t_{k+1}$ 
\beqa
E[J_N] &=&
\sum_k E[\rvB(t_{k+1})\Delta_{t_k}^{t_{k+1}}\rvB] 
\\
&=&
\sum_k
E[(\Delta_{0}^{t_{k+1}}\rvB)\Delta_{t_k}^{t_{k+1}}\rvB] 
\\
&=&
\sum_k
E[(\Delta_{t_k}^{t_{k+1}}\rvB)^2]
\\
&=&t
\eeqa



\beq
d[\rvB^2(t)]=
2\rvB(t)d\rvB(t)
+t
\eeq


\beq
[d\rvB(t)]^2 = dt
\eeq



\item $t_k^* = \frac{t_k + t_{k+1}}{2}$
Stratonovich integral

\end{enumerate}

For $\rvB\in\RR^n$,

\beq
\boxed{
d[\rvB_\alpha(t)\rvB_\beta(t)]=\delta(\alpha, \beta)
\left[
2\rvB_\alpha(t)d\rvB_\alpha(t)
+nt\right]}
\eeq

\beq
\boxed{
d[\rvB_\alpha(t)]d[\rvB_\beta(t)]
=Q_{\alpha, \beta}dt}
\eeq


\section{Some explicitly solvable examples}
Let $\mu, \nu, \alpha, \beta\in [n]$
\beq
d\rvx_\mu= f(\rvx, t)dt + L(\rvx, t)d\rvB_\mu(t)
\eeq


\beq
\pder{P}{t}= 
\pder{}{x_\mu}\left[-
Pf_\mu + \frac{1}{2}
\pder{}{ x_\nu}(PL_{\mu,\alpha}Q_{\alpha,\beta}L^T_{\beta,\nu})\right]
\eeq

\begin{itemize}

\item
{\bf Brownian motion} ($f_\mu=0$, $(LQL^T)_{\mu,\nu}=2D\delta(\mu, \nu)$)

\beq
dx_\mu =d\rvB_\mu
\eeq


\item {\bf Overdamped Langevin Equation}
($f_\mu=-\frac{1}{2}\pder{U}{x_\mu}$, $(LQL^T)_{\mu,\nu}=2D\delta(\mu, \nu)$)

\beq
dx_\mu = -\;\frac{1}{2}\pder{U}{x_\mu}dt + d\rvB_\mu
\eeq

\item {\bf Ornsteinâ€“Uhlenbeck process (a.k.a. Langevin equation)} ($f_\mu=-\lam x_\mu$, $(LQL^T)_{\mu,\nu}=2D\delta(\mu, \nu)$)

This is the same as the Langevin equation, if identify $\rvx$ with
the velocity of the 
particle and $\lam$ with the drag coefficient.


\beq
d\rvx = -\lam \rvx dt + d\rvB
\eeq

\item 
{\bf 1-dim ($n=1$) Black-Sholes} ($f=a x$, $(LQL^T)=(b\rvx)^2 q$)

\beq
d\rvx = a \rvx dt + b \rvx d\rvB
\eeq

\item {\bf 1-dim ($n=1$) General SDE}
($f=a x + c$, $(LQL^T)=(b\rvx + d)^2 q$)


\beq
d\rvx = [a(t)\rvx +c(t)]dt + [b(t)\rvx+ d(t)]d\rvB
\eeq


\beq
x(t) =\Psi(t, t_0)
\left(
x(t_0)
+
\int_{t_0}^{t}ds\;\Psi^{-1}(s, t_0)[c(s)-b(s)]
+
\int_{t_0}^{t}
\Psi^{-1}(s, t_0)d(s)d\rvW(s)
\right)
\eeq

\beq
\Psi(t, t_0)=
\exp\left(
\int_{t_0}^t ds\; \left[a(s)-\frac{1}{2}b^2(s)\right]
+
\int_{t_0}^t b(s) d\rvW(s)
\right)
\eeq



\end{itemize}


\section{Fockker-Planck Equation}


Consider $n$ dimensional case $\rvx, \rvW\in \RR^n$. Let $\mu, \nu,\alpha, \beta\in [n]$.
\beq
d\rvx_\mu= f(\rvx, t)dt + L(\rvx, t)d\rvB_\mu(t)
\eeq

\begin{claim}
\beq
d\phi=
\left[\pder{\phi}{t} +
\pder{\phi}{x_\mu} f_\mu +
\frac{\partial^2\phi}{\partial x_\mu\partial x_\nu}L_{\mu,\alpha}Q_{\alpha,\beta}L^T_{\beta,\nu}\right]dt
+
\pder{\phi}{x_\mu}L_{\mu,\nu}d\rvB_\nu
\eeq
\end{claim}
\proof






\beq
d\phi =
\pder{\phi}{t}dt
+
\sum_\mu \pder{\phi}{x_\mu} d\rvx_\mu
+\frac{1}{2}
\sum_\mu \sum_\nu \frac{\partial^2\phi}{\partial x_\mu\partial x_\nu}d\rvx_\mu d\rvx_\nu
\eeq


\beq
\pder{\phi}{x_\mu} d\rvx_\mu
=
\pder{\phi}{x_\mu} 
\left[
f_\mu dt + L_{\mu, \nu}d\rvB_\nu
\right]
\eeq

\beqa
\frac{\partial^2\phi}{\partial x_\mu\partial x_\nu}d\rvx_\mu d\rvx_\nu
&=&\frac{\partial^2\phi}{\partial x_\mu\partial x_\nu}
\left[
f_\mu dt + L_{\mu, \alpha}d\rvB_\alpha
\right]
\left[
f_\nu dt + L_{\nu, \beta}d\rvB_\beta
\right]
\\
&=&
\frac{\partial^2\phi}{\partial x_\mu\partial x_\nu}
L_{\mu, \alpha}  L_{\nu, \beta} d\rvB_\alpha d\rvB_\beta
\\
&=&
\frac{\partial^2\phi}{\partial x_\mu\partial x_\nu}
L_{\mu, \alpha}  L_{\nu, \beta} Q_{\alpha,\beta} dt
\eeqa

\beqa
d\phi &=&
\pder{\phi}{t}dt
+
\pder{\phi}{x_\mu} [f_\mu dt + L_{\mu,\nu}d\rvB_\nu]
+ \frac{1}{2}
\frac{\partial^2\phi}{\partial x_\mu\partial x_\nu}L_{\mu,\alpha}Q_{\alpha,\beta}L^T_{\beta,\nu}dt
\\
&=&
\left[\pder{\phi}{t} +
\pder{\phi}{x_\mu} f_\mu + \frac{1}{2}
\frac{\partial^2\phi}{\partial x_\mu\partial x_\nu}L_{\mu,\alpha}Q_{\alpha,\beta}L^T_{\beta,\nu}\right]dt
+
\pder{\phi}{x_\mu}L_{\mu,\nu}d\rvB_\nu
\eeqa

\qed

$\rvx(0)=x_0$

Example,  $n=1$, $\rvx=\rvB$, 
$\phi = \rvB^K$

$L=Q=1$, $f=0$

\beq
d(\rvB^K) = K(K-1) \rvB^{K-2}dt
+ K\rvB^{K-1}d\rvB
\eeq

$P(x, t)$
Fokker-Planck equation (FP) (a.k.a. Fokker-Planck-Kolgomrov equation)
\begin{claim} (FP)
\beq
\pder{P}{t}= 
\pder{}{x_\mu}\left[-
Pf_\mu + \frac{1}{2}
\pder{}{ x_\nu}(PL_{\mu,\alpha}Q_{\alpha,\beta}L^T_{\beta,\nu})\right]
\eeq

\end{claim}
\proof

\beq
\int dx^n\; P(x, t)\left[ \pder{\phi}{x_\mu}L_{\mu,\nu}d\rvB_\nu
\right]
=0
\eeq

Integration by parts

\beq
udv = d(uv)-(du)v 
\eeq

\beq
\int_{-\infty}^{+\infty}udv=
\underbrace{uv|_{-\infty}^{+\infty}}_{0}
\quad
-
\int_{-\infty}^{+\infty}(du)v 
\eeq



\beq
\int dt dx^n\; P(x, t)\frac{d\phi}{dt}=
\int dt dx^n\; P(x, t)
\left[\pder{\phi}{t} +
\pder{\phi}{x_\mu} f_\mu + \frac{1}{2}
\frac{\partial^2\phi}{\partial x_\mu\partial x_\nu}L_{\mu,\alpha}Q_{\alpha,\beta}L^T_{\beta,\nu}\right]
\eeq



\beq
-\int dt dx^n\; \phi\frac{dP}{dt}=
\int dt dx^n\;  \phi
\left[-\;\pder{P}{t} -
\pder{(Pf_\mu)}{x_\mu} + \frac{1}{2}
\frac{\partial^2 }{\partial x_\mu\partial x_\nu}(PL_{\mu,\alpha}Q_{\alpha,\beta}L^T_{\beta,\nu})\right]
\eeq


\qed


Diffusion equation, $n=1$, $f=0$, $L=1$, $Q=D>0$

\beq
dx = d\rvB
\eeq

\beq
\pder{P}{t} = D
\frac{\partial^2P}{\partial^2x}
\eeq

Overdamped Langevin Equation\footnote{
This equation arises from
Newton's equation $m\ddot{x}= -\lam\dot{x} + -U'(x)$ when the acceleration $\ddot{x}$ is negligible, so the drag force and potential force cancel each other.} 

\beq
dx_\mu = -\;\frac{1}{2}\pder{U}{x_\mu}dt + d\rvB
\eeq

\begin{claim}
For Brownian motion with drift,
if $Q =\frac{1}{\lam}>0$, then the steady state 
solution is

\beq
P(x) = \frac{e^{-\lam U(x)}}{Z}
\eeq
where 
\beq
Z = \int dx^n\;e^{-\lam U(x)}
 \eeq

\end{claim}
\proof
$L=1$, $\pder{P}{t}=0$
\beq
0= -
\pder{(Pf_\mu)}{x_\mu} + \frac{1}{2\lam}
\frac{\partial^2 P }{\partial x_\mu^2}
\eeq

$f_\mu =-\; \frac{1}{2}\pder{U}{x_\mu}$


\beq
0= \frac{1}{2}
\pder{}{x_\mu}\left(P\pder{U}{x_\mu} + \frac{1}{\lam}
\pder{P }{x_\mu}
\right)
\eeq


\beq
0=
\pder{}{x_\mu}\left(\lam e^{-\lam U}\pder{U}{x_\mu}+
\pder{e^{-\lam U}}{x_\mu}
\right) 
\eeq


\qed






\section{Martingale}

\beq
E\left[\rvx(t)|\rvx([0,t])=x([0,t])\right]= x(t)
\eeq

Brownian motion is a martingale

\beq
E[\;|\rvy(t_i)|\;] < \infty
\eeq

\beq
E[\rvy(t_{i+1})| \{\rvx(t_j) =x(t_j) \}_{j\leq i}] = x(t_i)
\eeq


$s\leq t$

\beq
E[\;|\rvy(t)|\;]<\infty
\eeq

\beq
E[\rvy(t)|\rvx(\leq s)=x(\leq s)]=y(s)
\eeq


Brownian motion is a martingale.
\beq
E[\rvB(t_{i+1})| \{\rvB(t_j) =B(t_j) \}_{j\leq i}] = B(t_i)
\eeq


It\^{o} integrals $\int L(\rvx(t), t)d\rvB(t)$
are martingales too, but Stratonovich 

\section{Chapman-Kolgomorov Equation}

Let $x(t_k) = x_k$

\beq
P(x_3|x_1) =\int dx^n_2\; P(x_3|x_2)P(x_2|x_1)
\eeq

\section{First and second order statistics}

\beq
m_\mu = E[\rvx(t)]
\eeq

\beq
C_{\mu, \nu}(t,s) = \av{\rvx_\mu(t), \rvx_\nu(s)}
\eeq

\beq
V_{\mu, \nu}(t) = C_{\mu, \nu}(t,t)
\eeq


\beq
dx_\mu = \left[a_\mu(t) + F_{\mu, \nu}(t)x_\nu \right] dt + 
L_{\mu, \nu}(t)d\rvB_\nu
\eeq

\beq
\frac{dm}{dt}=
a + Fm
\eeq

\beq
\frac{dV}{dt}= FV+VF^T + LQL^T
\eeq

Propagator
\beq
\pder{\Psi(\tau, t)}{\tau}  = F(\tau) \Psi(\tau, t)
\eeq

satisfies

\beq
\begin{array}{l}
\Psi(a, c) = \Psi(a, b)\Psi(b, c)
\\
\Psi^{-1}(a,b) = \Psi(b,a)
\\
\Psi(a,a)=1
\end{array}
\eeq




\beq
m(t) = \Psi(t, t_0)m(t_0) +\int_{t_0}^{t}d\tau\;
\Psi(t, \tau)a(t)
\eeq

\beq
V(t)=\Psi(t, t_0)V(t_0)\Psi^T(t, t_0)
+
\int_{t_0}^t d\tau\; \Psi(t, \tau)L(\tau)QL^T(\tau)
\Psi^T(t, \tau)
\eeq

If $P(x,t=0)$ is a Gaussian, $P(x, t)$ must be Gaussian too,
because the transformation is linear. Therefore,

\beq
P(x, t) = P(x(t))=
\caln(x(t); \mu=m(t), \Sigma^2=V(t))
\eeq

\beq
P(x(t)|x(s)) =\caln(x(t); \mu=m(t|s), \Sigma^2=V(t|s))
\eeq

where

\beq
m(t|s) =
\Psi(t,s)x(s)
+\int_{t_0}^t d\tau \Psi(t, \tau)a(\tau)
\eeq

\beq
V(t|s)=\int_s^td\tau\;
\Psi(t, \tau)L(\tau)QL^T(t, \tau)\Psi^T(t, \tau)
\eeq

\beq 
\Psi_k = \Psi(t_{k+1}, t_k)
\eeq

\beq
a_k = \int_{t_k}^{t_{k+1}}
d\tau\; \Psi(t_{k+1}, \tau)a(\tau)
\eeq

\beq
\Sigma_k=
\int_{t_k}^{t_{k+1}}d\tau\;
\Psi(t_{k+1}, \tau)L(\tau)QL^T(\tau)\Psi^T(t_{k+1}, \tau)
\eeq


\beq
P(\eps_k) = \caln(\eps_k; \mu=0, \Sigma=\Sigma_k)
\eeq

$x(t_k)=x_k$



\begin{figure}[h!]
$$
\xymatrix{
\ul{\eps}_3 \ar[d]
& \ul{\eps}_2 \ar[d]
& \ul{\eps}_1 \ar[d]
& \ul{\eps}_0\ar[d]
\\
\rvx_3 
& \rvx _2 \ar[l]
& \rvx_1 \ar[l]
& \rvx_0\ar[l]
}
$$
\caption{xx}
\label{fig-ist-2nd-order-bnet}
\end{figure}

\beq\color{blue}
\rvx_{k+1}= \Psi_k\rvx_k + a_k +\ul{\eps}_k
\eeq


\beq
\av{\rvx(t), \rvx^T(s)} = 
\left\{
\begin{array}{ll}
V(t)\Psi^T(s,t) &\text{if } t<s
\\
\Psi(t,s)V(s) & \text{if }t\geq s
\end{array}
\right.
\eeq

