\chapter{Kalman Filter}\label{ch-kalman}

This
chapter is based on Ref.\cite{wiki-kalman},
except we've replaced the
variables $F_t, w_t, v_t$ in that reference by 
$A_t, \xi_t,\zeta_t$, respectively.

A Kalman Filter (KF) is a special case of a
Hidden Markov Model. HMMs are
 discussed in Chapter \ref{ch-hmm}.

\begin{figure}[h!]
\centering
$$\xymatrix{
&\rvu_1\ar[dr]
&*++[F-o]{\rvxi_1}\ar[d]
&\rvu_1\ar[dr]
&\cdots
&\rvu_{t-1}\ar[dr]
&*++[F-o]{\rvxi_{t-1}}\ar[d]
&\rvu_t\ar[dr]|{B_t}
&*++[F-o]{\rvxi_{t}}\ar[d]^{Q_t}
\\
*++[F-o]{\rvx_0}\ar[d]\ar[rr]
&&*++[F-o]{\rvx_1}\ar[d]\ar[rr]
&&\cdots
&&*++[F-o]{\rvx_{t-1}}\ar[d]\ar[rr]_{A_t}
&&*++[F-o]{\rvx_{t}}\ar[d]^{H_t}
\\
\rvz_0
&&\rvz_1
&&\cdots
&&\rvz_{t-1}
&
&\rvz_{t}
\\
*++[F-o]{\rvzeta_0}\ar[u]
&&*++[F-o]{\rvzeta_1}\ar[u]
&&\cdots
&&*++[F-o]{\rvzeta_{t-1}}\ar[u]
&&*++[F-o]{\rvzeta_{t}}\ar[u]_{R_t}
}$$
\caption{Kalman Filter (KF) bnet.}
\label{fig-kal}
\end{figure}

Let 

$t=0, 1, 2, \dots , T-1$ be the time.

$\rvxi_t\in\RR^{nx},
 \rvzeta_t\in \RR^{nz}$ be
random variables that represent
hidden (unobserved)   external
Gaussian white noise.

$\rvx_t\in \RR^{nx}$ be
random variables that represent
the hidden (unobserved) true
state of the system.

$\rvu_t\in \RR^{nu}, 
\rvz_t\in \RR^{nz}$ be
random variables that represent
the measured (observed) 
state of the system.


The TPMs, printed in blue,
for the KF bnet Fig.\ref{fig-kal},
are as follows:

\beq\color{blue}
P(\xi_t)=\caln(\xi_t; 0, Q_t)
\;,
\eeq
where $Q_t$ is given.


\beq\color{blue}
P(x_t|x_{t-1}, u_t, \xi_t)=
\indi(x_t=A_tx_{t-1} + B_tu_t + \xi_t)
\;,
\eeq
where $A_t, B_tu_t$
are given. $P(x_t|x_{t-1}, u_t, \xi_t)$
 becomes $P(x_t)$
for $t=0$.

\beq\color{blue}
P(\zeta_t)=\caln(\zeta_t; 0, R_t)
\;,
\eeq
where $R_t$ is given.

\beq\color{blue}
P(z_t|x_t, \zeta_t)=
\indi(z_t=H_t x_t +  \zeta_t)
\;,
\eeq
where $H_t$ is given.


\section{Prediction
Problem}
Find $\hatx_t$ (the 
best possible estimate
of $x_t$)
and $P_t$ (the state of the 
filter at time $t$)
in terms of 
\begin{enumerate}
\item
$\hatx_{t-1}$
and $P_{t-1}$.
\item
 the 5 matrices
$\calm_t=(A_t,B_t,H_t,Q_t,R_t)$
\item
the observed  values of 
$z_t$ and $u_t$.

\end{enumerate}
See Fig.\ref{fig-kal-evol}.
For that figure,

\beq \color{blue}
P(\hatx_t, P_t | 
\hatx_{t-1}, P_{t-1},
\calm_t,
z_t,u_t)
=\delta(\hatx_t,?)
\delta(P_t, ?)
\;.
\eeq

\begin{figure}[h!]
\centering
$$\xymatrix{
\calm_0, \rvz_0,\rvu_0\ar[d]&
\calm_1, \rvz_1,\rvu_1\ar[d]&
\calm_2, \rvz_2,\rvu_2\ar[d]&
\calm_3, \rvz_3,\rvu_3\ar[d]
\\
\ul{\hatx}_0, 
\ul{P}_0\ar[r]&
\ul{\hatx}_1, 
\ul{P}_1\ar[r]&
\ul{\hatx}_2, 
\ul{P}_2\ar[r]&
\ul{\hatx}_3, 
\ul{P}_3
}$$
\caption{Evolution of
$\hatx_t, P_t$ for a KF.}
\label{fig-kal-evol}
\end{figure}

\section{
Solution} 

The algebraic solution
of
the prediction problem
for a KF 
is as follows.
See Fig.\ref{fig-kal-evol-plus}
for a bnet representation
of this algebraic
solution.

\begin{figure}[h!]
$$
\xymatrix@C=5pc{
P_{t-1}\ar[r]
&P_{t|t-1}\ar[r]\ar[rd]
&P_t
\\
&&
K_t\ar[u]
\\
u_{t-1}
&
&u_t\ar[ld]|{B_t}
\\
\hatx_{t-1}\ar[r]^{A_t}
&\hatx_{t|t-1}\ar[r]^1
\ar[d]_{-H_t}
&\hatx_t\ar[d]^{-H_t}
\\
\tilde{y}_{t-1}
&\tilde{y}_{t|t-1}\ar[ru]|{K_t}
&\tilde{y}_t
\\
z_{t-1}
&
&z_t\ar[lu]^1
\ar[u]_1
}
$$
\caption{Bnet representation
of the algebraic
solution of
the prediction 
problem for a KF.}
\label{fig-kal-evol-plus}
\end{figure}


Define $\eta_{t|t}=\eta_t$ for 
$\eta=\hatx, P$.

\begin{itemize}
\item{\bf Initial Conditions} $\hatx_0, P_0$
\item{\bf A priori estimates}

a priori state estimate
\beq
\hatx_{t| t-1} =
\underbrace{ A_t
\hatx_{t-1}
 + B_t u_{t}
}_{x_t-\xi_t}
\eeq

a priori covariance estimate
\beq
P_{t| t-1} =
 A_t 
P_{t-1}
 A_t^T +
 Q_t
\eeq

\item{\bf A posteriori estimates}



Optimal Kalman gain $K_t$

\beq
S_t = H_t 
P_{t| t-1} 
H_t^T +
 R_t
\eeq

\beqa
K_t &=&
P_{t| t-1}
H_t^T
 S_t^{-1}
\\
&=&
 P_{t| t-1}
H_t^T
\left[
H_t 
P_{t| t-1} 
H_t^T +
 R_t
\right]^{-1}
\eeqa


a posteriori state estimate



\beq
\tilde{y}_{t|t-1}=
z_t - 
H_t\hatx_{t| t-1}
\eeq




\beqa
\hatx_{t} &=&
 \hatx_{t| t-1} +
 K_t\tilde{y}_{t|t-1}
\\
&=&
(1-K_tH_t)\hatx_{t| t-1} +
 K_t\underbrace{z_t}_{H_t x_t + \zeta_t}
\quad\text{(interpolation formula)}
\label{eq-kal-interpol-f}
\eeqa

\beq
\tilde{y}_{t}=
z_t - 
H_t\hatx_{t}
\eeq



a posteriori covariance estimate
\beq
P_{t} = \left(I -
 K_t H_t\right) 
P_{t|t-1} 
\eeq



\end{itemize}



\section{Simple Example}

$r_t$ position, $v_t$ velocity, $a_t$
acceleration of point particle.

\beq
x_t=A x_{t-1} + B u_t +\xi_t
\eeq

\beq
x_t= 
\left[
\begin{array}{c}
r_t
\\
v_t
\end{array}
\right]
\;,\quad u_t=a_t
\eeq

\beq
A=
\left[
\begin{array}{cc}
1 & \Delta t
\\
0& 1
\end{array}\right]
\;,\quad
B=
\left[
\begin{array}{c}
\frac{1}{2}(\Delta t)^2
\\
\Delta t
\end{array}\right]
\eeq

\beq
z_t = H x_t + \zeta_t
\eeq

\beq
H =
\left[
\begin{array}{cc}
1&0
\end{array}
\right]
\eeq

\section{Invariants}

Note that

\beq
x_t-\hatx_{t|t-1}=\xi_t
\eeq

\beqa
x_t-\hatx_t&=&
(1-K_tH_t)(x_t-\hatx_{t|t-1})-K_t\zeta_t
\\
&=&
(1-K_tH_t)\xi_t-K_t\zeta_t
\label{eq-kalm-delta-xt}
\eeqa

\beqa
\tilde{y}_{t|t-1}&=&
\underbrace{z_t}_{H_t x_t + \zeta_t} - 
H_t\hatx_{t| t-1}
\\
&=&
H_t
\xi_t +\zeta_t
\eeqa


\beqa
\tilde{y}_{t} &=&
\underbrace{z_t}_{H_t x_t + \zeta_t} - H_t
\hatx_{t}
\\
&=&
H_t(x_t-\hatx_t)+\zeta_t
\\
&=&
H_t(1-K_tH_t)\xi_t 
+(1-H_tK_t)\zeta_t
\eeqa
$(x_t-\hatx_{t|t-1})$, $(x_t-\hatx_t)$,
$\tilde{y}_{t|t-1}$ and $\tilde{y}_t$
are called {\bf residuals}.
Since $\xi_t$ and $\zeta_t$
have zero mean
value,


\beq
E[\rvx_t -\ul{\hatx}_t]
=
E[\rvx_t -\ul{\hatx}_{t|t-1}]=0
\eeq

\beq
E[\tilde{\rvy}_t]
=E[\tilde{\rvy}_{t|t-1}]
=0
\eeq
These zero mean value identities
are called {\bf invariants}.

\section{Derivation
of Solution}

First, some notational
conventions. Let

\beq
Cov(\rva)_{i,j}=\av{\rva_i, \rva_j}
\eeq

\beq
Cov(\rva)=\av{\rva, \rva^T}=
\av{\rva,tp.}
\eeq
\beq
[A,B]_+= AB+B^TA^T
\eeq

\beq
A + tp. = A + A^T
\eeq
$tp.$ stands for transpose.

Now define
\beq
P_t= Cov(\rvx_t -\ul{\hatx}_t)
\eeq

\beq
P_{t|t-1}=Cov(\rvx_t-
\ul{\hatx}_{t|t-1})
\eeq

\beq
S_t=Cov(\tilde{\rvy}_{t|t-1})
\eeq
It follows that


\begin{align}
P_t &=
\av{\rvx_t-\hat{\rvx}_t,tp.}
\\
&=
\av{(1-K_tH_t)(\rvx_t-\hat{\rvx}_{t|t-1})
-K_t\rvzeta_t
,tp.}\quad\text{(by Eq.(\ref{eq-kalm-delta-xt}))}
\\
&= 
\av{(1-K_tH_t)(\rvx_t-
\hat{\rvx}_{t|t-1}), tp.}
+
\av{K_t\rvzeta_t,tp.}
\;\text{($\rvzeta_t$ 
uncorrelated with $(\rvx_t-
\hat{\rvx}_{t|t-1})$)}
\\
&=
(1-K_tH_t)
\underbrace{\av{\rvx_t-
\hat{\rvx}_{t|t-1},tp.}}_{
P_{t|t-1}
}
(1-K_tH_t)^T
+K_t
\underbrace{\av{\rvzeta_t,tp.}}_{R_t}
K_t^T
\\
&=
P_{t|t-1}
-
[K_t H_t, P_{t|t-1}]_{+}
+K_t
\underbrace{
\left(
H_tP_{t|t-1} H_t^T + R_t\right)}_
{S_t}
K_t^T
\end{align}

Next we find the optimal
Kalman gain $K_t$
by minimizing 
with respect to $K_t$
the 
following mean squared error.

\beqa
\cale &=& \sum_i E[
(\rvx_t-\hat{\rvx}_t)_i^2]
\\
&=&
\tr E\left[(\rvx_t-\hat{\rvx}_t)
(\rvx_t-\hat{\rvx}_t)^T\right]
\\
&=&
\tr P_t
\\
&=&
\tr
\left(
P_{t|t-1}
-
[K_t H_t, P_{t|t-1}]_{+}
+K_t
S_t
K_t^T
\right)
\eeqa
If we set to zero the variation of
$\cale$ when $K_t$ varies, we get

\beq
0=\delta\cale=
\tr\left[\left(
-P_{t|t-1}H_t^T
+K_tS_t
\right)\delta K_t^T \right]+tp.
\eeq
Hence

\beq
-P_{t|t-1}H_t^T
+K_t S_t=0
\eeq

\beq
K_t=P_{t|t-1}H_t^T S_t^{-1}
\eeq
