\chapter{Selection Bias Removal}
\label{ch-sb-removal}

 

\begin{figure}[h!]
$$
\begin{array}{ccc}
\xymatrix{
&\rvbeta\ar[dl]\ar[d]\ar[dr]&\rvs\ar[l]
\\
&&
}
&\quad\quad&
\xymatrix{
\ar[dr]&\ar[d]&\ar[dl]
\\
&\rvbeta&\rvs\ar[l]
}
\\
(a)\text{ root node selector} 
&& (b)\text{ leaf node selector}
\end{array}
$$
\caption{}
\label{}
\end{figure}

\beq\color{blue}
P(\rvbeta=\beta|s)=
\left\{
\begin{array}{ll}
\delta(\beta, \beta_0)&\text{if $s=0$}
\\
P^*(\beta)&\text{if $s=1$}
\end{array}
\right.
\eeq

\beq\color{blue}
P(\rvbeta=\beta|s, pa^-(\rvbeta))=
\left\{
\begin{array}{ll}
P(\beta)&\text{if $s=0$}
\\
P^*(\beta|pa^-(\beta))&\text{if $s=1$}
\end{array}
\right.
\eeq


{\bf S-Recoverable (selection recoverable)}
                                                       

\hrule
\begin{enumerate}
\item Selection Bias (SB)
\beq\xymatrix{
\rvx\ar[rr]\ar[dr]
&&\rvy\ar[dl]
\\
&\rvbeta&\rvs\ar[l]
}\eeq

\hrule\item Confounding
\beq\xymatrix{
&*++[F-o]{\rvbeta}
\ar[dl]\ar[dr]
&\rvs\ar[l]
\\
\rvx\ar[rr]
&&\rvy
}\eeq


\hrule\item SB of treatment.  $Q=P(y|x)$ recoverable
\beq\xymatrix{
\rvx\ar[rr]\ar[dr]
&&\rvy
\\
&\rvbeta&\rvs\ar[l]
}\eeq

\hrule\item SB of outcome. $Q=P(y|x)$ NOT recoverable
\beq\xymatrix{
\rvx\ar[rr]
&&\rvy\ar[dl]
\\
&\rvbeta&\rvs\ar[l]
}\eeq


\hrule\item $Q=P(y|x)$ recoverable
\beq\xymatrix{
\rvx\ar[rr]\ar[dr]
&&\rvy
\\
\rvz\ar[u]\ar[r]
&\rvbeta&\rvs\ar[l]
}\eeq

\hrule\item $Q=P(y|x)$ NOT recoverable
\beq\xymatrix{
&\rvw\ar[dl]\ar[dr]
\\
\rvx\ar[rr]\ar[dr]
&&\rvy
\\
\rvz\ar[u]\ar[r]
&\rvbeta&\rvs\ar[l]
}\eeq

\hrule\item $Q=P(y|\cald x=x)$ recoverable if condition on $\rvx, \rvw$
\beq\xymatrix{
\rvx\ar[dr]\ar[rr]
&&\rvy\ar[dl]
\\
&\rvw\ar[d]
\\
&\rvbeta&\rvs\ar[l]
}\eeq

\hrule\item $Q=P(y|\cald x=x)$ recoverable if condition on $\rvx, \rvw_2$
\beq\xymatrix{
\rvw_1\ar[rr]\ar[d]
&&\rvw_2\ar[d]\ar[ddl]
\\
\rvx\ar[rr]
&&\rvy
\\
&\rvbeta&\rvs\ar[l]
}\eeq

\hrule\item $Q=P(y|\cald x=x)$ recoverable if condition on $\rvx$
\beq\xymatrix{
&&*++[F-o]{\rvc}
\ar[dl]\ar[dr]
\\
\rvw_1\ar[r]\ar[d]
&\rvw_2\ar[r]
&\rvx\ar[r]
&\rvy
\\
\rvbeta&\rvs\ar[l]
}\eeq
\end{enumerate}