\chapter{LDEN with feedback loops: 
COMING SOON}\label{ch-LDEN-feedback}

\begin{figure}[h!]
$$
\begin{array}{cc}
\xymatrix@R=4pc{
\rvx_0\ar@(ul,ur)@[green]@{-->}[]^{\beta_{0|0}}
\ar@[green]@{-->}@/_3pc/[d]_{\beta_{1|0}}
\ar[d]^{\alp{1|0}}
\\
\rvx_1\ar@(dl,dr)@[green]@{-->}[]_{\beta_{1|1}}
\ar@[green]@{-->}@/_3pc/[u]_{\beta_{0|1}}
}
&
\xymatrix{
\rvx_0^{[1]}\ar[d]
\ar@[green][r]\ar@[green][rd]
&\rvx_0^{[2]}\ar[d]
\ar@[green][r]\ar@[green][rd]
&\rvx_0^{[3]}\ar[d]
\\
\rvx_1^{[1]}\ar@[green][r]\ar@[green][ru]
&\rvx_1^{[2]}\ar@[green][r]\ar@[green][ru]
&\rvx_1^{[3]}
}
\\
(a)&(b)
\end{array}
$$
\caption{
LDEN diagram with two $\rvx_j$
nodes
(exogenous nodes $\rvu_j$
not shown).}
\label{fig-LDEN-fb-2}
\end{figure}



\beqa
\rvx_0^{[t+1]} &=& \underbrace{\sum_{j=0}^1\beta_{0|j}\rvx_j^{[t]}
 }_{\text{from past}}
 +\rvu_0^{[t+1]}
\\
\rvx_1^{[t+1]} &=&
\underbrace{\sum_{j=0}^1\beta_{1|j}\rvx_j^{[t]}
}_{\text{from past}}
+  \alp_{1|0}\rvx_0^{[t+1]} + \rvu_1^{[t+1]}
\eeqa

$\rvx^{[0]}_j=0$ for all $j$.

\beq
\rvx^{[t+1]}_j
\maparrow{\calz}
z
\left(
\TIL{\rvx}_j(z)
-z
\rvx^{[0]}_j
\right)= z\TIL{\rvx}_j(z)
\eeq

\beqa
z\TIL{\rvx}_0(z) &=& \sum_{j=0}^1\beta_{0|j}
\TIL{\rvx}_j(z)
 +z\TIL{\rvu}_0(z)
\\
z\TIL{\rvx}_1(z) &=&
\sum_{j=0}^1\beta_{1|j}\TIL{\rvx}_j(z)
+  \alp_{1|0}z\TIL{\rvx}_0(z) + z\TIL{\rvu}_1(z)
\eeqa
 
\beq
\TIL{x}=\left[
\begin{array}{c}
\TIL{x}_0
\\
\TIL{x}_1
\end{array}
\right],
\quad
\TIL{u}=\left[
\begin{array}{c}
\TIL{u}_0
\\
\TIL{u}_1
\end{array}
\right]
,\quad
A=\left[
\begin{array}{cc}
0
&0
\\
\alp_{1|0}
&0
\end{array}
\right]
,\quad
B=\left[
\begin{array}{cc}
\beta_{0|0}
&\beta_{0|1}
\\
\beta_{1|0}
&\beta_{1|1}
\end{array}
\right]
\eeq

\beq
0 = \underbrace{(\frac{1}{z}B+A)}_
{M}\TIL{x} + \TIL{u}
\eeq

\beq
M = LU
\eeq

\beq
L = 
\left[
\begin{array}{cc}
-1
&0
\\
l_{1,0}
&-1
\end{array}
\right],
\quad
U = 
\left[
\begin{array}{cc}
u_{0,0}
&u_{0,1}
\\
0
&u_{1,1}
\end{array}
\right]
\eeq

\beq
\TIL{\rvX} = U\TIL{\rvx}
\eeq

\beq
\TIL{\rvX}=(L+1)\TIL{\rvX} + \TIL{u}
\eeq

\beq
[C_{\TIL{\rvx}}]_{i,j} =\av{\rvx_i, \rvx_j},
\quad  
[C_{\TIL{\rvX}}]_{i,j} =\av{\rvX_i, \rvX_j}
\eeq

\beqa
C_{\TIL{\rvx}}=\av{\TIL{\rvx}, \TIL{\rvx}^T}
&=&
U^{-1}\av{\TIL{\rvX}, \TIL{\rvX}^T}(U^{-1})^T
\\
&=&
U^{-1}C_{\TIL{\rvX}}(U^{-1})^T
\eeqa

\beq
C_{\TIL{\rvX}}=
UC_{\TIL{\rvX}}U^T
\eeq

\beq
LU = \frac{1}{z}B + A
\eeq
