
\chapter{IN PROGRESS: Generative Adversarial Networks, Ensemble GANs}
\begin{refsection}
Bayesian GAN, 
 Ref.\cite{wilson2017} (2017)

Replace $\theta_a$ by $\vtheta_a$ and 
$\theta'_a$ by $\vtheta'_a$ for $a=G,D$



\beq
\delta V(\vtheta_G, \vtheta_D)=0
\eeq

\beq
 \partial_{\vtheta_G}V(\vtheta_G, \vtheta_D)=
 \partial_{\vtheta_D}V(\vtheta_G, \vtheta_D)=0
\eeq

\beq
V_{opt}=\min_{\vtheta_G}\max_{\vtheta_D} V(\vtheta_G, \vtheta_D)
\eeq

\beq
P(\vtheta_G)=\prod_i P(\theta_G[i])
\eeq

\beq
P(\vtheta_D)=\prod_i P(\theta_D[i])
\eeq


\beq
P(\vecu)=\prod_i P(u[i])
\eeq

\beq
P(\vecr)=\prod_i P(r[i])
\eeq


\beq
P(f[i]|\vecu, \vtheta_G)= \prod_i\delta[f[i], G(u[i],\vtheta_G)]
\eeq

\beq
P(c[i]|\vecf, \vtheta_D) = \delta(c[i], \ol{D}(f[i], \vtheta_D))
\eeq

\beq
P(d[j]|\vecr, \vtheta_D)= \delta(d[j], D(r[j], \vtheta_D))
\eeq


\beq
P(V| \vecd,  \vecc)=
\delta(V, \frac{1}{N}\ln \prod_{i,j}(c[i]d[j]))
\eeq
where $N=nsam(\rvr)nsam(\rvu)$







$\eta_G, \eta_D> 0$, maximize wrt $\theta_D$, 
minimize wrt $\theta_G$
\beq
P(\theta'_G|V,\vtheta_G )=
\delta(\vtheta'_G, \vtheta_G - \eta_G 
\partial_{\vtheta_G}V)
\eeq

\beq
P(\theta'_D|V,\vtheta_D )=
\delta(\vtheta'_D, \vtheta_D + \eta_D 
\partial_{\vtheta_D}V)
\eeq


\hrule
Emulated B net

\beq
P(\vtheta_G)=\;\prod_i P(\theta_G[i])
\eeq

\beq
P(\vtheta_D)=\;\prod_i P(\theta_D[i])
\eeq


\beq
P(u[i]|\vtheta_G, \vtheta_D)=  
\ol{D}(G(u[i],\vtheta_G), \vtheta_D)
\eeq


\beq
P(r[i]|\vtheta_D)=  
D(r[i], \vtheta_D)
\eeq

\beq
P(V| \vecd,  \vecc)=
\delta(V, \prod_{i,j,a,b}(u[i]r[j]\theta_G[a]\theta_D[b]))
\eeq



$\eta_G, \eta_D > 0$, maximize wrt $\theta_D$, 
minimize wrt $\theta_G$
\beq
P(\vtheta'_G|V,\vtheta_G )=
\prod_i \delta(\theta'_G[i], \theta_G[i] - \eta_G 
\partial_{\theta_G[i]}\ln V)
\eeq

\beq
P(\vtheta'_D|V,\vtheta_D )=\prod_i
\delta(\theta'_D[i], \theta_D[i] + \eta_D 
\partial_{\theta_D[i]}\ln V)
\eeq

\beq
P(\vecr, \vecu, \vtheta_G, \vtheta_D)=
\prod_{i,j,a,b}
\left\{
P(\theta_G[a])P(\theta_D[b])\\
 \frac{D(r[i], \theta_D[b])}{\lam(\theta_D[b])}
\frac{\ol{D}(G(u[j],\theta_G[a]),\theta_D[b]))}
{\ol{\lam}(\theta_G[a], \theta_D[b])}
\right\}
\eeq


$N=nsam(\vecr)nsam(\vecu)
nsam(\vtheta_G)nsam(\vtheta_D)$

\beq
\ln P(\vecr, \vecu, \vtheta_G, \vtheta_D) =
N\left\{
\begin{array}{l}
-H(P_{\ul{\theta}_D})+ \sum_{r,\theta_D}P(r)P(\theta_D)
\ln \frac{D(r, \theta_D)}{\lam(\theta_D)}
\\
-H(P_{\ul{\theta}_G})+ \sum_{u,\theta_G,\theta_D}P(u)
P(\theta_G)P(\theta_D)\ln
\frac{\ol{D}(G(u,\theta_G),\theta_D)}{\ol{\lam}(\theta_G, \theta_D)}
\end{array}
\right.
\eeq

\beq
\ln P(\vecr, \vecu) =
N\left\{
\begin{array}{l}
 \sum_{r}P(r)
\ln \sum_{\theta_D}P(\theta_D)\frac{D(r, \theta_D)}{\lam(\theta_D)}
\\
+ \sum_{u}P(u)
\ln \sum_{\theta_D, \theta_G}
P(\theta_G)P(\theta_D)
\frac{\ol{D}(G(u,\theta_G),\theta_D)}{\ol{\lam}(\theta_G, \theta_D)}
\end{array}
\right.
\eeq

\beqa
V(\vtheta_G, \vtheta_D) &=&\frac{1}{N} \ln P(\vtheta_G, \vtheta_D|\vecr,\vecu,)\\&=&
\frac{1}{N} [
\ln P(\vecr,\vecu,\vtheta_G, \vtheta_D)
-\ln P(\vecr,\vecu)]
\eeqa



\printbibliography[heading=subbibliography]
\end{refsection}
